heap_lang/tactics.v
@@ -32,6 +32,7 @@ Ltac reshape_expr e tac :=
     | Case ?e0 ?e1 ?e2                => add_item (CaseCtx e1 e2) vs K e0
     | AllocN ?e (Val ?v)              => add_item (AllocNLCtx v) vs K e
     | AllocN ?e1 ?e2                  => add_item (AllocNRCtx e1) vs K e2
+    | Free ?e                         => add_item FreeCtx vs K e
     | Load ?e                         => add_item LoadCtx vs K e
     | Store ?e (Val ?v)               => add_item (StoreLCtx v) vs K e
     | Store ?e1 ?e2                   => add_item (StoreRCtx e1) vs K e2
